chore: Split files + refactor Definitions

theories/SimplyTypedLambdaCalculus/StrongNormalisation.v
@@ -1,111 +1,13 @@
-From FormArith Require Export Base.
-
-From Autosubst Require Import Autosubst.
-
-Inductive term : Type :=
-| Var (n : var)
-| App (s t : term)
-| Lam (s : {bind term}).
-
-Instance Ids_term : Ids term. derive. Defined.
-Instance Rename_term : Rename term.  derive. Defined.
-Instance Subst_term : Subst term. derive. Defined.
-
-Instance SubstLemmas_term : SubstLemmas term. derive. Defined.
-
-Lemma var_subst:
-  forall (x:var) (sigma : var -> term), (Var x).[sigma] = sigma x.
-Proof.
-  now intros x sigma.
-Qed.
-
-Inductive step : term -> term -> Prop :=
-| Step_beta (s s' t : term) : s' = s.[t .: ids] -> step (App (Lam s) t) s'
-| Step_app1 (s s' t : term) : step s s' -> step (App s t) (App s' t)
-| Step_app2 (s t t' : term) : step t t' -> step (App s t) (App s t')
-| Step_lam (s s' : term) : step s s' -> step (Lam s) (Lam s').
-
-Lemma step_subst :
-  forall (t t' : term) (sigma : var -> term),
-    step t t' -> step t.[sigma] t'.[sigma].
-Proof.
-  induction t; intros t' sigma Hstep.
-  - easy.
-  - inversion Hstep; subst.
-    + simpl. constructor. asimpl. reflexivity.
-    + simpl. constructor. auto.
-    + simpl. constructor. auto.
-  - inversion Hstep. subst. simpl.
-    constructor. auto.
-Qed.
-
-Inductive type :=
-| Base
-| Arr (A B : type).
-
-Inductive types (Gamma : var -> type) : term -> type -> Prop :=
-| Types_var (x : var) (A : type) : Gamma x = A -> types Gamma (Var x) A
-| Types_app (s t : term) (A B : type) :
-  types Gamma s (Arr A B) -> types Gamma t A ->
-  types Gamma (App s t) B
-| Types_lam (s : term) (A B : type) : types (A .: Gamma) s B -> types Gamma (Lam s) (Arr A B).
-
-Lemma type_weakening :
-  forall (Gamma : var -> type) (s : term) (A : type),
-    types Gamma s A ->
-    (forall Delta xi, Gamma = xi >>> Delta -> types Delta s.[ren xi] A).
-Proof.
-  intros Gamma s A H. induction H; intros; simpl; econstructor; auto.
-  - rewrite H0 in H. auto.
-  - asimpl. apply IHtypes. rewrite H0. asimpl. reflexivity.
-Qed.
+From FormArith.SimplyTypedLambdaCalculus Require Import Definitions.
 
 Create HintDb typingSTLC.
 
 Hint Resolve type_weakening : typingSTLC.
 Hint Resolve Types_app : typingSTLC.
 Hint Resolve Types_var : typingSTLC.
-
-
-
-#[export] Hint Extern 3 (@types _ _ _) => asimpl : typingSTLC.
-
-
-
-Lemma type_subst :
-  forall (Gamma Delta : var -> type) (s : term) (A : type) (sigma : var -> term),
-    types Gamma s A ->
-    (forall (x:var) , types Delta (sigma x) (Gamma x)) ->
-    types Delta s.[sigma] A.
-Proof.
-  intros Gamma Delta s. revert Gamma Delta. induction s; intros; simpl; inversion H; subst.
-  - auto.
-  - eauto with typingSTLC.
-  - constructor. eapply IHs.
-    + eassumption.
-    + intros [| x]; eauto with typingSTLC.
-Qed.
-
 Hint Resolve type_subst : typingSTLC.
 
-Lemma type_pres :
-  forall (Gamma : var -> type) (s t : term) (A : type),
-    types Gamma s A -> step s t -> types Gamma t A.
-Proof.
-  intros Gamma s. revert Gamma. induction s; intros; asimpl; auto.
-  - inversion H0.
-  - inversion H0; subst.
-    + inversion H; subst. inversion H3; subst.
-      eapply type_subst.
-      * eassumption.
-      * intros [|x]; eauto with typingSTLC.
-    + inversion H. subst. eauto 3 with typingSTLC.
-    + inversion H. subst. eauto 3 with typingSTLC.
-  - inversion H0. subst. inversion H. subst.
-    constructor. apply IHs; assumption.
-Qed.
-
-(** STRONG NORMALISATION PROOF *)
+#[export] Hint Extern 3 (@types _ _ _) => asimpl : typingSTLC.
 
 Inductive sn : term -> Prop :=
 | Strong (t : term) :
