theories/SimplyTypedLambdaCalculus/Definitions.v
@@ -1,0 +1,136 @@
+From FormArith Require Export Base.
+
+From Autosubst Require Export Autosubst.
+
+Inductive term : Type :=
+  | Var (n: var)
+  | App (s t: term)
+  | Lam (s: {bind term}).
+
+Instance Ids_term: Ids term. derive. Defined.
+Instance Rename_term: Rename term. derive. Defined.
+Instance Subst_term: Subst term. derive. Defined.
+Instance SubstLemmas_term: SubstLemmas term. derive. Defined.
+
+
+Inductive step: term -> term -> Prop :=
+  | Step_beta (s s' t: term): s' = s.[t .: ids] -> step (App (Lam s) t) s'
+  | Step_app1 (s s' t: term): step s s' -> step (App s t) (App s' t)
+  | Step_app2 (s t t': term): step t t' -> step (App s t) (App s t')
+  | Step_lam (s s': term): step s s' -> step (Lam s) (Lam s').
+
+Lemma step_subst (t t': term) (sigma: var -> term):
+  step t t' -> step t.[sigma] t'.[sigma].
+Proof.
+  revert t' sigma.
+
+  induction t as [ | ? IHs ? IHt | s IHs ].
+  - inversion 1.
+
+  - inversion 1; subst; simpl.
+    + apply Step_beta.
+      asimpl.
+      reflexivity.
+
+    + apply Step_app1.
+      apply IHs.
+      assumption.
+
+    + apply Step_app2.
+      apply IHt.
+      assumption.
+
+  - inversion 1; subst; simpl.
+    apply Step_lam.
+    apply IHs.
+    assumption.
+Qed.
+
+
+Inductive type :=
+  | Base
+  | Arr (A B: type).
+
+Inductive types (Gamma: var -> type): term -> type -> Prop :=
+  | Types_var (x: var) (A: type):
+      Gamma x = A -> types Gamma (Var x) A
+
+  | Types_app (s t: term) (A B: type) :
+      types Gamma s (Arr A B) ->
+      types Gamma t A ->
+      types Gamma (App s t) B
+
+  | Types_lam (s: term) (A B: type):
+      types (A .: Gamma) s B ->
+      types Gamma (Lam s) (Arr A B).
+
+Lemma type_weakening (gamma: var -> type) (s: term) (A: type):
+  types gamma s A ->
+    forall (gamma': var -> type) (x': var -> var),
+      gamma = x' >>> gamma' -> types gamma' s.[ren x'] A.
+Proof.
+  induction 1 as [ ? ? ? H | ? ? ? A ? _ IH1 _ IH2 | ? ? ? ? _ IH ]; intros ? ? H'; simpl.
+  - apply Types_var.
+    rewrite H' in H; simpl in H.
+    assumption.
+
+  - apply Types_app with A.
+    + now apply IH1.
+    + now apply IH2.
+
+  - apply Types_lam; asimpl.
+    apply IH.
+    now rewrite H'; asimpl.
+Qed.
+
+Lemma type_subst (gamma gamma': var -> type) (s: term) (A: type) (sigma: var -> term):
+  types gamma s A ->
+  (forall (x: var) , types gamma' (sigma x) (gamma x)) ->
+  types gamma' s.[sigma] A.
+Proof.
+  revert gamma gamma' A sigma.
+
+  induction s as [ | ? IH1 ? IH2 | ? IH ]; intros gamma gamma' ? ? Hgamma Hgamma'; simpl.
+  all: inversion Hgamma as [ | ? ? A' | ? A' ]; subst.
+
+  - apply Hgamma'.
+  - apply Types_app with A'.
+    + now apply IH1 with gamma.
+    + now apply IH2 with gamma.
+  - apply Types_lam.
+    apply IH with (A' .: gamma); [ assumption |].
+    intros [| x ]; asimpl.
+    + now apply Types_var.
+    + now apply type_weakening with gamma'.
+Qed.
+
+Lemma type_preservation (gamma: var -> type) (s t: term) (A: type):
+  types gamma s A -> step s t -> types gamma t A.
+Proof.
+  revert gamma t A.
+
+  induction s as [ | ? IH1 ? IH2 | ? IH ]; intros gamma ? ? Hgamma Hgamma'; asimpl.
+  all: inversion Hgamma; subst.
+  all: inversion Hgamma' as [ s' | | | ]; subst.
+
+  all: match goal with
+       | H: types _ _ (Arr ?A _) |- _ => rename A into A'
+       end.
+
+  - match goal with
+    | H: types gamma (Lam s') _ |- _ => inversion H; subst
+    end.
+
+    apply type_subst with (A' .: gamma); [ assumption |].
+    intros [| x ]; asimpl; [ assumption |].
+    now apply Types_var.
+
+  - apply Types_app with A'; [| assumption ].
+    now apply IH1.
+
+  - apply Types_app with A'; [ assumption |].
+    now apply IH2.
+
+  - apply Types_lam.
+    now apply IH.
+Qed.
